\section{Basic Concepts}

\paragraph{Observables}
An observable is a Hermitian operator whose orthonormal eigenvectors form a basis.

\paragraph{The Postulates of Quantum Mechanics}
The postulates of quantum mechanics are:
\begin{itemize}
	\item At any fixed time the state of a physical system is specified by a ket in Hilbert space.
	\item Every measurable physical quantity corresponds to an operator on Hilbert space. This is a Hermitian observable. The possible outcomes of a measurement are the eigenvalues of $A$.
	\item The probability of measuring the value $a$ of operator $A$ in a normalized state $\ket{\Psi}$ is $P(a) = \expval{P_{a}}{\Psi}$, where $P_{a}$ is the projector onto the subspace corresponding to the eigenvalue $a$ given by $P_{a} = \dyad{a}{a}$.
	\item If a measurement of an observable $A$ gives an outcome $a$, the state of the system immediately after the measurement is the projection of the state onto the subspace with eigenvalue $a$.
	\item The time evolution of a state is governed by the Schrödinger equation.
\end{itemize}

\paragraph{Consequences of the Probability Picture}
The form of writing the projection operator implies $P(a) = \abs{\bra{a}\ket{\Psi}}^{2}$, or $P(a)\dd{a} = \abs{\bra{a}\ket{\Psi}}^{2}\dd{a}$ in the continuous case. In order for the probability interpretation to be consistent, i.e. for the sum of all probabilities to amount to $1$, it must hold that $\bra{\Psi}\ket{\Psi} = 1$.

\paragraph{Expectation Values}
Expectation values are given by
\begin{align*}
	\expval{A} = \sum aP(a) = \sum a\expval{P_{a}}{\Psi} = \bra{\Psi}\sum a\ket{a}\bra{a}\ket{\Psi} = \expval{A}{\Psi}.
\end{align*}

\paragraph{Physical States}
Modifying a state by a phase factor $e^{i\alpha}$ does not change any expectation values.

\paragraph{Mixed States}

\paragraph{Density Matrix}
The density matrix is defined as
\begin{align*}
	\rho = \op{\Psi}{\Psi}.
\end{align*}
It has some cool properties. For instance:
\begin{align*}
	&\tr{\rho} = \sum\limits_{n}\expval{\rho}{n} = \ev**{\sum\limits_{n}\op{n}{n}}{\psi} = \braket{\Psi} = 1, \\
	&\adj{\rho} = \rho, \\
	&\expval{A} = \sum\limits_{n, m}\braket{\Psi}{n}\mel{n}{A}{m}\braket{m}{\Psi} = \sum\limits_{n, m}\braket{m}{\Psi}\braket{\Psi}{n}\mel{n}{A}{m} = \sum\limits_{n, m}\mel{m}{\rho}{n}\mel{n}{A}{m} = \tr(\rho A), \\
	&\rho^{2} = \rho.
\end{align*}
Note that the latter is only true for pure states. Mixed states have a density matrix of the form
\begin{align*}
	\rho = \sum\limits_{j}P_{j}\op{\Psi_{j}}{\Psi_{j}}.
\end{align*}

\paragraph{The Time Evolution Operator}
Suppose that there exists an operator $u_{t'}(t)$ which evolves $\ket{\Psi(t')}$ to $\ket{\Psi(t)}$. Such an operator should satisfy
\begin{itemize}
	\item $u_{t'}(t) = u_{t''}(t)u_{t'}(t'')$ for consistency.
	\item $u_{t'}(t)$ is unitary to preserve the normalization.
	\item $u_{t}(t) = 1$.
\end{itemize}
Inserting this into the Schrödinger equation yields
\begin{align*}
	i\hbar\dv{t}u_{t^{\prime}}(t)\ket{\Psi(t^{\prime})} = Hu_{t^{\prime}}(t)\ket{\Psi(t^{\prime})}, \\
	i\hbar\del{t}{t^{\prime}} = Hu_{t^{\prime}}(t).
\end{align*}
In the case of a time-independent Hamiltonian, the solution must be of the form $u_{t^{\prime}}(t) = u(t - t^{\prime})$, and the equation above can be integrated to yield
\begin{align*}
	u_{t^{\prime}}(t) = e^{-i\frac{t - t^{\prime}}{\hbar}H}.
\end{align*}

\paragraph{Symmetries in Quantum Mechanics}
A symmetry in a quantum mechanics context is any transformation acting on Hilbert space that leaves all probabilities invariant.

\paragraph{Wigner's Theorem}
Wigner's theorem states that any operator that is a symmetry is either unitary or anti-unitary ($\mel{\Phi}{\adj{U}U}{\Psi} = \braket{\Psi}{\Phi}$).

\paragraph{Transformation of Operators}
Consider a symmetry operator $u$. In order for this to be a symmetry, it must also act on all operators according to $A\to uA\adj{u}$.

\paragraph{Time Evolution From Symmetry}
Consider some system with time translation symmetry - that is, any system for which time translations do not change the theory. Introduce the transformation operator
\begin{align*}
	u_{\tau}\ket{\Psi(t)} = \ket{\Psi(t + \tau)}.
\end{align*}
This transformation is a smooth map acting on a manifold - namely, Hilbert space. Hence we can use the language of Lie algebra to treat this (if you know nothing about Lie algebra, pretend that I didn't write this and carry on. If you want some reference material, please look at my summary of SI2360). We expand the transformation operator around the identity as
\begin{align*}
	u_{\tau} = 1 - i\frac{\tau}{\hbar}H
\end{align*}
for some operator $H$. The requirement that this be unitary yields $\adj{H} - H = 0$, and hence the generator $H$ is self-adjoint. By continuous application of this we obtain
\begin{align*}
	u_{\tau} = e^{-i\frac{\tau}{\hbar}H}.
\end{align*}
This reproduces the Schrödinger equation, tying it all together neatly. It also demonstrates that the Hamiltonian generates time translation in a mathematical sense.

\paragraph{Space Translation}
Consider the space operator $x^{i}$. A space translation $u$ transforms $x^{i}$ to $x^{i} + a^{i}$, meaning $ux^{i}\adj{u} = x^{i} + a^{i}$. Expanding the translation around the identity yields
\begin{align*}
	u = 1 + i\frac{a^{i}}{\hbar}p_{i}
\end{align*}
for some operator $p_{i}$. The requirement that $u$ be unitary implies that $p$ is self-adjoint. The transformation rule yields
\begin{align*}
	(1 + i\frac{a^{i}}{\hbar}p_{i})x^{i}(1 - i\frac{a^{i}}{\hbar}p_{i}) = x^{i} + i\frac{a^{i}}{\hbar}\pb{p_{i}}{x^{i}}
\end{align*}
and the requirement
\begin{align*}
	\comm{p_{i}}{x^{i}} = -i\hbar.
\end{align*}

\paragraph{Time Evolution of the Density Matrix}
The time evolution of the density matrix is given by
\begin{align*}
	\rho(t) = \sum P_{i}u_{t_{0}}(t)\ket{\Psi_{i}}\bra{\Psi_{i}}\adj{u_{t_{0}}(t)} = u_{t_{0}}(t)\rho(t_{0})\adj{u_{t_{0}}(t)}.
\end{align*}
This implies
\begin{align*}
	i\hbar\dv{t}\rho = Hu_{t_{0}}(t)\rho(t_{0})\adj{u_{t_{0}}(t)} - u_{t_{0}}(t)\rho(t_{0})\adj{u_{t_{0}}(t)}H = H\rho(t) - \rho(t)H = \comm{H}{\rho}.
\end{align*}

\paragraph{The Heisenberg Equation}
Heisenberg's outlook starts from preserving expectation values under time translations in such a way that all (total) time evolution is contained in the operators, arriving at the transformation rule
\begin{align*}
	A_{\text{H}} = \adj{u_{t_{0}}}(t)A_{\text{S}}u_{t_{0}}(t).
\end{align*}
$A_{\text{H}}$ is the operator according to Heisenberg and $A_{\text{S}}$ is the operator according to Schrödinger. We now have
\begin{align*}
	i\hbar\dv{t}\expval{A_{\text{H}}} &= -\adj{u_{t_{0}}}(t)HA_{\text{S}}u_{t_{0}}(t) + \adj{u_{t_{0}}}(t)(i\hbar\del{t}{A_{\text{S}}})u_{t_{0}}(t) + \adj{u_{t_{0}}}(t)A_{\text{S}}Hu_{t_{0}}(t) \\
	                                  &= -\adj{u_{t_{0}}}(t)Hu_{t_{0}}(t)\adj{u_{t_{0}}}(t)A_{\text{S}}u_{t_{0}}(t) + \adj{u_{t_{0}}}(t)(i\hbar\del{t}{A_{\text{S}}})u_{t_{0}}(t) + \adj{u_{t_{0}}}(t)A_{\text{S}}u_{t_{0}}(t)\adj{u_{t_{0}}}(t)Hu_{t_{0}}(t) \\
	                                  &= -H_{\text{H}}A_{\text{H}} + \adj{u_{t_{0}}}(t)(i\hbar\del{t}{A_{\text{S}}})u_{t_{0}}(t) + A_{\text{H}}H_{\text{H}} \\
	                                  &= -{H_{\text{H}}}\comm{A_{\text{H}}} + (i\hbar\del{t}{A_{\text{S}}})_{\text{H}}.
\end{align*}

\paragraph{Propagators}
The probability amplitude at some point $x$ at time $t$ is given by
\begin{align*}
	\Psi(x, t) = \braket{x}{\Psi(t)} = \mel{x}{u_{0}(t)}{\Psi(0)} = \integ{}{}{x^{\prime}}{\mel{x}{u_{0}(t)}{x^{\prime}}\braket{x^{\prime}}{\Psi(0)}}.
\end{align*}
Defining the propagator $G_{x^{\prime}, t^{\prime}}(x, t) = \mel{x}{u_{t^{\prime}}(t)}{x^{\prime}}$, we arrive at
\begin{align*}
	\Psi(x, t) = \integ{}{}{x^{\prime}}{G_{x^{\prime}, 0}(x, t)\braket{x^{\prime}}{\Psi(0)}} = \integ{}{}{x^{\prime}}{G_{x^{\prime}, 0}(x, t)\Psi(x^{\prime}, 0)}.
\end{align*}
Hence the propagator acts as a Green's function with respect to time, in some sense.

\paragraph{Arriving at Path Integrals}
The general propagator of some state is given by
\begin{align*}
	G_{x^{\prime}, t^{\prime}}(x, t) = \sum\limits_{\gamma}G_{\gamma; x^{\prime}, t^{\prime}}(x, t),
\end{align*}
where the summation is performed over all possible paths $\gamma$ between the two points.

Suppose now that the time evolution is divided into steps such that
\begin{align*}
	u_{t^{\prime}}(t) = \prod\limits_{k = 1}^{n}u_{t_{k - 1}}(t_{k}),\ t_{0} = t^{\prime},\ t_{n} = t,\ t_{k} - t_{k - 1} = \delta t.
\end{align*}
Then
\begin{align*}
	G_{x^{\prime}, t^{\prime}}(x, t) = \mel**{x}{\prod\limits_{k = 1}^{n}u_{t_{k - 1}}(t_{k})}{x^{\prime}}.
\end{align*}
For every $k$ we now introduce an identity according to
\begin{align*}
	G_{x^{\prime}, t^{\prime}}(x, t) &= \mel**{x}{\prod\limits_{k = 1}^{n}u_{t_{k - 1}}(t_{k})\integ{}{}{x_{k}}{\op{x_{k - 1}}{x_{k - 1}}}}{x^{\prime}} \\
	                                 &= \mel**{x}{\prod\limits_{k = 1}^{n}\integ{}{}{x_{k}}{u_{t_{k - 1}}(t_{k})\op{x_{k - 1}}{x_{k - 1}}}}{x^{\prime}} \\
	                                 &= \int\prod\limits_{k = 1}^{n}\dd{x_{k}}\mel{x_{k}}{u_{t_{k - 1}}(t_{k})}{x_{k - 1}}.
\end{align*}
The time translation operator has the form $u_{t_{k - 1}}(t_{k}) = e^{-i\frac{\Delta t}{\hbar}H}$. For a Hamiltonian of the form $H = \frac{p^{2}}{2m} + V(\vb{x})$, the terms do not necessarily commute. However, to second order we have
\begin{align*}
	e^{\alpha A}e^{\alpha B} &= \left(1 + \alpha A + \frac{1}{2}\alpha^{2}A^{2} + \dots\right)\left(1 + \alpha B + \frac{1}{2}\alpha^{2}B^{2} + \dots\right), \\
	e^{\alpha(A + B)}  &= 1 + \alpha A + \alpha B + \frac{1}{2}\alpha^{2}(A^{2} + B^{2} + AB + BA) + \dots, \\
	           &= e^{A}e^{B}\left(1 - \frac{1}{2}\alpha^{2}AB + \frac{1}{2}\alpha^{2}BA + \dots\right) \\
	           &= e^{\alpha A}e^{\alpha B}e^{\frac{1}{2}\alpha^{2}\comm{A}{B}}.
\end{align*}
Ignoring the second-order term yields
\begin{align*}
	G_{x^{\prime}, t^{\prime}}(x, t) &= \int\prod\limits_{k = 1}^{n}\dd{x_{k}}\mel{x_{k}}{e^{-i\frac{\Delta t}{\hbar}(T + V)}}{x_{k - 1}} \\
	                                 &= \int\prod\limits_{k = 1}^{n}\dd{x_{k}}e^{-i\frac{\Delta t}{\hbar}V(x_{k - 1})}\mel{x_{k}}{e^{-i\frac{\Delta t}{\hbar}T}}{x_{k - 1}} \\
	                                 &= \int\prod\limits_{k = 1}^{n}\dd{x_{k}}e^{-i\frac{\Delta t}{\hbar}V(x_{k - 1})}\mel**{x_{k}}{e^{-i\frac{\Delta t}{\hbar}T}\integ{}{}{p_{k}}{\op{p_{k}}{p_{k}}}}{x_{k - 1}} \\
	                                 &= \int\prod\limits_{k = 1}^{n}\dd{x_{k}}e^{-i\frac{\Delta t}{\hbar}V(x_{k - 1})}\mel**{x_{k}}{\integ{}{}{p_{k}}{e^{-i\frac{\Delta t}{\hbar}T}\op{p_{k}}{p_{k}}}}{x_{k - 1}} \\
	                                 &= \int\prod\limits_{k = 1}^{n}\dd{x_{k}}e^{-i\frac{\Delta t}{\hbar}V(x_{k - 1})}\integ{}{}{p_{k}}{e^{-i\frac{\Delta t}{2m\hbar}p_{k}^{2}}\braket{x_{k}}{p_{k}}\braket{p_{k}}}{x_{k - 1}} \\
	                                 &= \int\prod\limits_{k = 1}^{n}\dd{x_{k}}e^{-i\frac{\Delta t}{\hbar}V(x_{k - 1})}\integ{}{}{p_{k}}{e^{-i\frac{\Delta t}{2m\hbar}p_{k}^{2}}\frac{1}{2\pi\hbar}e^{i\frac{p_{k}(x_{k} - x_{k - 1})}{\hbar}}} \\
	                                 &= \int\prod\limits_{k = 1}^{n}\dd{x_{k}}e^{-i\frac{\Delta t}{\hbar}V(x_{k - 1})}e^{i\frac{m}{2\hbar\Delta t}(x_{k} - x_{k - 1})^{2}}\frac{1}{2\pi\hbar}\integ{}{}{p_{k}}{e^{-i\frac{\Delta t}{2m\hbar}\left(p_{k} - \frac{m}{\Delta t}(x_{k} - x_{k - 1})\right)^{2}}} \\
	                                 &= \int\prod\limits_{k = 1}^{n}\dd{x_{k}}e^{-i\frac{\Delta t}{\hbar}V(x_{k - 1})}e^{i\frac{m}{2\hbar\Delta t}(x_{k} - x_{k - 1})^{2}}\sqrt{\frac{m}{2\pi^{2}\hbar\Delta ti}}\integ{}{}{v_{k}}{e^{-v_{k}^{2}}} \\
	                                 &= \int\prod\limits_{k = 1}^{n}\dd{x_{k}}e^{-i\frac{\Delta t}{\hbar}V(x_{k - 1})}e^{i\frac{m}{2\hbar\Delta t}(x_{k} - x_{k - 1})^{2}}\sqrt{\frac{m}{2\pi\hbar\Delta ti}} \\
	                                 &= \int\prod\limits_{k = 1}^{n}\dd{x_{k}}\sqrt{\frac{m}{2\pi\hbar\Delta ti}}e^{i\frac{1}{\hbar}\sum\limits_{k = 1}^{n}\left(\frac{1}{2}m\left(\frac{x_{k} - x_{k - 1}}{\Delta t}\right)^{2} - V(x_{k - 1})\right)\Delta t}.
\end{align*}
In the continuous limit the exponent becomes
\begin{align*}
	i\frac{1}{\hbar}\integ{}{}{t}{\frac{1}{2}m\dot{x}^{2} - V(x)} = i\frac{S}{\hbar}
\end{align*}
where $S$ is the action. The remaining factor, termed the measure, is
\begin{align*}
	D(x(t)) = \lim\limits_{\Delta t \to 0}\prod\limits_{k = 1}^{n}\dd{x_{k}}\sqrt{\frac{m}{2\pi\hbar\Delta ti}}.
\end{align*}
Finally the propagator is given by
\begin{align*}
	G_{x^{\prime}, t^{\prime}}(x, t) &= \int D(x(t))e^{-i\frac{S}{\hbar}}.
\end{align*}
This is termed the path integral.

As a side note, if the action is large compared to $\hbar$, the action varies strongly, causing destructive interference from all paths except for the one such that
\begin{align*}
	\fdv{S}{x} = 0.
\end{align*}
This is Hamilton's principle, the fundamental postulate of classical mechanics.