\section{Useful Mathematics}

\paragraph{A Useful Commutation Relation}
You might happen upon commutation relations of the form $\comm{f(A)}{B}$ show up. We would like to try to simplify it for the particular case where $\comm{A}{B} = C$, where $C$ is some operator commuting with $A$. To do this, we first study $\comm{A^{n}}{B}$ in a general case. We have
\begin{align*}
	\comm{A^{n}}{B} = A\comm{A^{n - 1}}{B} + \comm{A}{B}A^{n - 1},
\end{align*}
prompting us to find this commutator by induction. For $n = 2$ we have
\begin{align*}
	\comm{A^{2}}{B} = A\comm{A}{B} + \comm{A}{B}A.
\end{align*}
For $n = 3$ we obtain
\begin{align*}
	\comm{A^{3}}{B} = A\comm{A^{2}}{B} + \comm{A}{B}A^{2} = A(A\comm{A}{B} + \comm{A}{B}A) + \comm{A}{B}A^{2} = A^{2}\comm{A}{B} + A\comm{A}{B}A + \comm{A}{B}A^{2}.
\end{align*}
A suitable induction hypothesis looks to be
\begin{align*}
	\comm{A^{n}}{B} = \sum\limits_{k = 1}^{n}A^{n - k}\comm{A}{B}A^{k - 1}.
\end{align*}
Assuming it to be true, we have
\begin{align*}
	\comm{A^{n + 1}}{B} &= A\comm{A^{n}}{B} + \comm{A}{B}A^{n} \\
	                    &= A\sum\limits_{k = 1}^{n}A^{n - k}\comm{A}{B}A^{k - 1} + \comm{A}{B}A^{n} \\
	                    &= \sum\limits_{k = 1}^{n}A^{n + 1 - k}\comm{A}{B}A^{k - 1} + \comm{A}{B}A^{n} \\
	                    &= \sum\limits_{k = 1}^{n + 1}A^{n + 1 - k}\comm{A}{B}A^{k - 1},
\end{align*}
proving the hypothesis by induction.

Now we write
\begin{align*}
	f(A) = \sum\limits_{n = 0}^{\infty}\frac{1}{n!}f_{n}A^{n}
\end{align*}
to obtain
\begin{align*}
	\comm{f(A)}{B} &= \comm{\sum\limits_{n = 0}^{\infty}\frac{1}{n!}f_{n}A^{n}}{B} \\
	               &= \sum\limits_{n = 0}^{\infty}\frac{1}{n!}f_{n}\comm{A^{n}}{B} \\
	               &= \sum\limits_{n = 0}^{\infty}\frac{1}{n!}f_{n}\sum\limits_{k = 1}^{n}A^{n - k}\comm{A}{B}A^{k - 1}.
\end{align*}
Assuming $\comm{A}{B}$ to commute with $A$, we have
\begin{align*}
	\comm{f(A)}{B} &= \sum\limits_{n = 0}^{\infty}\frac{1}{n!}f_{n}A^{n - 1}\comm{A}{B}\sum\limits_{k = 1}^{n} \\
	               &= \comm{A}{B}\sum\limits_{n = 1}^{\infty}\frac{1}{(n - 1)!}f_{n}A^{n - 1} \\
	               &= \comm{A}{B}\sum\limits_{m = 0}^{\infty}\frac{1}{m!}f_{m + 1}A^{m} \\
	               &= \comm{A}{B}\dv{f}{A}.
\end{align*}